Define the new horizontal composition

games/ATS.v
@@ -1,77 +1,135 @@
-Require Import LogicalRelations.
+Require Export LogicalRelations.
+Require Export Games.
 Require Import KLR.
 Require Import List.
-Require Import Games.
 
-(** ** Alternating transition systems *)
 
-Record ats {GA GB S K} :=
-  {
-    step : S -> S -> Prop;
-    suspend : S -> pmove GA GB * K -> Prop;
-    resume : K -> omove GA GB -> S -> Prop;
-    refuse : K -> question GB -> Prop;
-  }.
+(** * Alternating transition systems *)
 
-Arguments ats : clear implicits.
+Module ATS.
 
-Section SIM.
-  Context {GA1 GA2} (GRA : grel GA1 GA2).
-  Context {GB1 GB2} (GRB : grel GB1 GB2).
-  Context {S1 S2} (RS : klr (gworld GRA GRB) S1 S2).
-  Context {K1 K2} (RK : klr (gworld GRA GRB) K1 K2).
+  (** ** Definition *)
 
-  Record sim (α1 : ats GA1 GB1 S1 K1) (α2 : ats GA2 GB2 S2 K2) :=
+  Record ats {GA GB S K} :=
     {
-      step_sim :
-        (|= RS ++> k1 set_le RS)%rel (step α1) (step α2);
-      suspend_sim :
-        (|= RS ++> k1 set_le (<> * RK))%rel (suspend α1) (suspend α2);
-      resume_sim :
-        (|= RK ++> [] -> k1 set_le RS)%rel (resume α1) (resume α2);
-      refuse_sim :
-        (|= RK ++> [] -> k impl)%rel (refuse α1) (refuse α2);
+      step : S -> S -> Prop;
+      suspend : S -> pmove GA GB * K -> Prop;
+      resume : K -> omove GA GB -> S -> Prop;
+      refuse : K -> question GB -> Prop;
     }.
-End SIM.
 
-(** ** Strategies *)
+  Arguments ats : clear implicits.
 
-Record strategy {GA GB : game} :=
-  {
-    state : Type;
-    cont : Type;
-    transitions :> ats GA GB state cont;
-    init_cont : cont;
-  }.
 
-Record ref {GA1 GA2} (GRA: grel GA1 GA2) {GB1 GB2} (GRB: grel GB1 GB2) σ1 σ2 :=
-  {
-    state_rel : klr (gworld GRA GRB) (state σ1) (state σ2);
-    cont_rel : klr (gworld GRA GRB) (cont σ1) (cont σ2);
-    ref_transitions : sim GRA GRB state_rel cont_rel σ1 σ2;
-    ref_init_cont : cont_rel nil (init_cont σ1) (init_cont σ2);
-  }.
+  (** ** Simulations *)
 
-(** ** Traces *)
+  Section SIM.
+    Context {GA1 GA2} (GRA : grel GA1 GA2).
+    Context {GB1 GB2} (GRB : grel GB1 GB2).
+    Context {S1 S2} (RS : klr (gworld GRA GRB) S1 S2).
+    Context {K1 K2} (RK : klr (gworld GRA GRB) K1 K2).
 
-Inductive strace {GA GB S K} (α : ats GA GB S K) : S -> play GA GB -> Prop :=
-  | strace_step s s' t :
-      step α s s' ->
-      strace α s' t ->
-      strace α s (tau :: t)
-  | strace_suspend s m k t :
-      suspend α s (m, k) ->
-      ktrace α k t ->
-      strace α s (ext (pm m) :: t)
-with ktrace {GA GB S K} (α : ats GA GB S K) : K -> play GA GB -> Prop :=
-  | ktrace_nil k :
-      ktrace α k nil
-  | ktrace_omove k m :
-      ktrace α k (ext (om m) :: nil)
-  | ktrace_resume k m s t :
-      resume α k m s ->
-      strace α s t ->
-      ktrace α k (ext (om m) :: t)
-  | ktrace_refuse k m :
-      refuse α k m ->
-      ktrace α k (ext (oq m) :: refused :: nil).
+    Record sim (α1 : ats GA1 GB1 S1 K1) (α2 : ats GA2 GB2 S2 K2) :=
+      {
+        sim_step :
+          (|= RS ++> k1 set_le RS)%rel (step α1) (step α2);
+        sim_suspend :
+          (|= RS ++> k1 set_le (<> * RK))%rel (suspend α1) (suspend α2);
+        sim_resume :
+          (|= RK ++> [] -> k1 set_le RS)%rel (resume α1) (resume α2);
+        sim_refuse :
+          (|= RK ++> [] -> k impl)%rel (refuse α1) (refuse α2);
+      }.
+  End SIM.
+
+  Global Instance step_sim :
+    Monotonic
+      (@step)
+      (forallr GRA, forallr GRB, forallr RS, forallr RK,
+       sim GRA GRB RS RK ++> |= RS ++> k1 set_le RS).
+  Proof.
+    firstorder.
+  Qed.
+
+  Global Instance suspend_sim :
+    Monotonic
+      (@suspend)
+      (forallr GRA, forallr GRB, forallr RS, forallr RK,
+       sim GRA GRB RS RK ++> |= RS ++> k1 set_le (<> * RK)).
+  Proof.
+    firstorder.
+  Qed.
+
+  Global Instance resume_sim :
+    Monotonic
+      (@resume)
+      (forallr GRA, forallr GRB, forallr RS, forallr RK,
+       sim GRA GRB RS RK ++> |= RK ++> [] -> k1 set_le RS).
+  Proof.
+    repeat intro. eapply sim_resume; eauto.
+  Qed.
+
+  Global Instance refuse_sim :
+    Monotonic
+      (@refuse)
+      (forallr GRA, forallr GRB, forallr RS, forallr RK,
+       sim GRA GRB RS RK ++> |= RK ++> [] -> k impl).
+  Proof.
+    firstorder.
+  Qed.
+
+  (** Identity and composition *)
+
+  Global Instance sim_id G S K :
+    Reflexive (sim (@grel_id G) (@grel_id G) (k (@eq S)) (k (@eq K))).
+  Proof.
+    split.
+    - intros w s _ [ ]. rstep. reflexivity.
+    - intros w s _ [ ]. rstep. reflexivity || admit.
+    - intros w k _ [ ]. reflexivity || admit.
+    - intros w k _ [ ]. reflexivity || admit.
+  Admitted.
+
+  (* some version of:
+  Global Instance sim_compose {GA GB GC GRAB GRBC A B C RAB RBC RAC} :
+    (forall wab wbc, RDecompose (RAB wab) (RBC wbc) (RAC (wab, wbc))) ->
+    (forall wab wbc, RCompose (RAB wab) (RBC wbc) (RAC (wab, wbc))) ->
+    @RCompose (ats GA A) (ats GB B) (ats GC C)
+      (sim GRAB RAB)
+      (sim GRBC RBC)
+      (sim (grel_compose GRAB GRBC) RAC).
+   *)
+
+
+  (** ** Nonbranching *)
+
+  
+
+
+  (** ** Traces *)
+
+  Inductive strace {GA GB S K} (α : ats GA GB S K) : S -> play GA GB -> Prop :=
+    | strace_step s s' t :
+        step α s s' ->
+        strace α s' t ->
+        strace α s (tau :: t)
+    | strace_suspend s m k t :
+        suspend α s (m, k) ->
+        ktrace α k t ->
+        strace α s (ext (pm m) :: t)
+  with ktrace {GA GB S K} (α : ats GA GB S K) : K -> play GA GB -> Prop :=
+    | ktrace_nil k :
+        ktrace α k nil
+    | ktrace_omove k m :
+        ktrace α k (ext (om m) :: nil)
+    | ktrace_resume k m s t :
+        resume α k m s ->
+        strace α s t ->
+        ktrace α k (ext (om m) :: t)
+    | ktrace_refuse k m :
+        refuse α k m ->
+        ktrace α k (ext (oq m) :: refused :: nil).
+
+End ATS.
+
+Notation ats := ATS.ats.
