games/MultiChannel.v
@@ -3,10 +3,10 @@ Require Import KLR.
 Require Import Classical.
 Require Import ClassicalChoice.
 Require Import DecidableClass.
-Require Import RTS.
+Require Import ATS.
 
 
-(** * Multi-channel game *)
+(** * Side-by-side composition *)
 
 Module Pow.
 
@@ -14,118 +14,77 @@ Module Pow.
 
   Definition g G I :=
     {|
-      move := I * move G;
+      question := I * question G;
+      answer := I * answer G;
     |}.
 
+  Definition r {G1 G2} (GR : grel G1 G2) (I : Type) :=
+    Build_grel (g G1 I) (g G2 I)
+      (grel_world GR)
+      (k eq * question_rel GR)
+      (k eq * answer_rel GR).
+
   Infix "^" := g : game_scope.
+  Infix "^" := r : grel_scope.
 
-  (** ** Simulations *)
+  Definition mko {GA GB I} (i : I) (m : omove GA GB) : omove (GA ^ I) (GB ^ I) :=
+    match m with
+      | inl ma => inl (i, ma)
+      | inr mq => inr (i, mq)
+    end.
 
-  Section GREL.
-    Context {G1 G2} (GR : grel G1 G2) (I : Type).
+  Definition mkp {GA GB I} (i : I) (m : pmove GA GB) : pmove (GA ^ I) (GB ^ I) :=
+    match m with
+      | inl mq => inl (i, mq)
+      | inr ma => inr (i, ma)
+    end.
 
-    Inductive world :=
-      mkw (w : I -> GR) (i : I).
+  (** ** Transition system *)
 
-    Inductive acc : relation world :=
-      mkw_acc w i w' i' :
-        (forall j, j <> i' -> w' j = w j) ->
-        w i' ~> w' i' ->
-        acc (mkw w i) (mkw w' i').
+  Section ATS.
+    Context {GA GB I} {S K : I -> Type} (α : forall i, ats GA GB (S i) (K i)).
 
-    Inductive mrel : klr world (move (G1 ^ I)) (move (G2 ^ I)) :=
-      mrel_intro w i m1 m2 :
-        move_rel GR (w i) m1 m2 ->
-        mrel (mkw w i) (i, m1) (i, m2).
-          
-    Definition r :=
-      {|
-        gworld := world;
-        gacc := acc;
-        ginitw := fun '(mkw w i) => forall j, ginitw GR (w j);
-        move_rel := mrel;
-      |}.
-  End GREL.
+    Inductive state :=
+      st (i : I) (s : S i) (k : forall j, i <> j -> K j).
 
-  Arguments mkw {G1 G2 GR I}.
-  Arguments acc {G1 G2 GR I}.
+    Definition cont :=
+      forall i : I, K i.
 
-  Definition getw {G1 G2 GR I} : @r G1 G2 GR I -> GR :=
-    fun '(mkw f i) => f i.
+    Inductive step : relation state :=
+      step_intro i s s' k :
+        ATS.step (α i) s s' ->
+        step (st i s k) (st i s' k).
 
-End Pow.
+    Inductive suspend : state -> pmove (GA ^ I) (GB ^ I) * cont -> Prop :=
+      suspend_intro i s k m ki k' :
+        ATS.suspend (α i) s (m, ki) ->
+        (forall j Hj, k' j = k j Hj) ->
+        k' i = ki ->
+        suspend (st i s k) (mkp i m, k').
 
-Infix "^" := Pow.g : game_scope.
-Infix "^" := Pow.r : grel_scope.
+    Inductive resume : cont -> omove (GA ^ I) (GB ^ I) -> state -> Prop :=
+      resume_intro i k m s :
+        ATS.resume (α i) (k i) m s ->
+        resume k (mko i m) (st i s (fun j _ => k j)).
 
+    Inductive refuse : cont -> question (GB ^ I) -> Prop :=
+      refuse_intro i k m :
+        ATS.refuse (α i) (k i) m ->
+        refuse k (i, m).
 
-(** * Relational maps *)
+    Definition of :=
+      ATS.Build_ats (GA ^ I) (GB ^ I) state cont step suspend resume refuse.
 
-(** A common pattern when defining operators which operate over
-  multiple components is that we keep keep a vector with an entry for
-  each component. When the system is suspended, all entries will be
-  continuations. When the system is running, most entries will still
-  be continuations, but the entry for the currently running component
-  will be a state instead.
+  End ATS.
 
-  This file defines a data structure which facilitates keeping track
-  of such composite states, and establishing simulations between
-  them. *)
-
-(** A type of maps with relational update operations. *)
-
-Module RMap.
-
-  (** ** Definition *)
-
-  (** We continuously switch between two kinds of map. The "unfocused"
-    maps are used for continuations and are simple functions. *)
-
-  Definition unfocused I A :=
-    I -> A.
-
-  (** The "focused" map are focused on a specific index, which takes a
-    value from a different type. This is used for running states. *)
-
-  Inductive focused I A B :=
-    foc (i : I) (b : B) (f : forall j, i <> j -> A).
-
-  Arguments foc {I A B}.
-
-  (** ** Operations *)
-
-  (** The map is initialized in an unfocused state with a constant
-    value. *)
-
-  Definition init {I A} (a : A) : unfocused I A :=
-    (fun _ => a).
-
-  (** The first operation will focus it on a specific component and
-    update the value. *)
-  
-  Inductive focus {I A B} i: unfocused I A -> A * (B -> focused I A B) -> Prop :=
-    focus_intro f :
-      focus i f (f i, fun b => foc i b (fun j _ => f j)).
-
-  (** A focused map can be updated as follows. *)
-
-  Inductive update {I A B} (b' : B) : focused I A B -> I * B * focused I A B -> Prop :=
-    update_intro i b f :
-      update b' (foc i b f) (i, b, foc i b' f).
-
-  (** Later, we can unfocus the map again by providing a replacement
-    value for [f i] *)
-
-  Inductive unfocus {I A B}: focused I A B -> I * B * (A -> unfocused I A) -> Prop :=
-    unfocus_intro i b f f' :
-      (forall a j Hj, f' a j = f j Hj) ->
-      (forall a, f' a i = a) ->
-      unfocus (foc i b f) (i, b, f').
+  Arguments state : clear implicits.
+  Arguments cont : clear implicits.
 
   (** ** Monotonicity *)
 
   (** We can build KLRs for these two kinds of maps. *)
 
+  (*
   Section REL.
     Context {G1 G2} (GR : grel G1 G2) (I : Type).
     Context {A1 A2} (RA : klr GR A1 A2).
@@ -164,72 +123,9 @@ Module RMap.
                        ((<> RA@@[Pow.getw]) ++> <> unfocused_r))).
     Admitted.
   End REL.
+*)
 
-End RMap.
+End Pow.
 
-
-(** * Multi-component transition systems *)
-
-Module MC.
-
-  (** ** Definition *)
-
-  Section RTS.
-    Context {G : game} {I S : Type}.
-
-    Definition state :=
-      RMap.focused I (RTS.cont G S) S.
-    
-    (** *** Continuations *)
-
-    Inductive liftk (k: RMap.unfocused I (RTS.cont G S)): RTS.cont (G^I) state :=
-      liftk_intro i ki q r f :
-        RMap.focus i k (ki, f) ->
-        ki q r ->
-        liftk k (i, q) (RTS.resumption_map f r).
-
-    (** *** Steps *)
-
-    Inductive step (α : I -> rts G S) : rts (G ^ I) state :=
-      | step_internal i si si' s s' :
-          RMap.update si' s (i, si, s') ->
-          α i si (RTS.internal si') ->
-          step α s (RTS.internal s')
-      | step_interacts i p si ki s f :
-          RMap.unfocus s (i, si, f) ->
-          α i si (RTS.interacts p ki) ->
-          step α s (RTS.interacts (G := G ^ I) (i, p) (liftk (f ki)))
-      | step_diverges s i si f :
-          RMap.unfocus s (i, si, f) ->
-          α i si RTS.diverges ->
-          step α s RTS.diverges
-      | step_goes_wrong s i si f :
-          RMap.unfocus s (i, si, f) ->
-          α i si RTS.goes_wrong ->
-          step α s RTS.goes_wrong.
-
-  End RTS.
-
-  Arguments state : clear implicits.
-
-  (** ** Simulations *)
-
-  Global Instance liftk_sim :
-    Monotonic
-      (@liftk)
-      (forallr GR, forallr - @ I, forallr R : klr _,
-         |= RMap.unfocused_r GR I (RTS.cont_le GR R) ++>
-            RTS.cont_le (GR ^ I) (RMap.focused_r GR I (RTS.cont_le GR R) R)).
-  Proof.
-  Admitted.
-
-  Global Instance step_sim :
-    Monotonic
-      (@step)
-      (forallr GR, forallr - @ I, forallr R : klr _,
-         (- ==> RTS.sim GR R) ++>
-         RTS.sim (GR ^ I) (RMap.focused_r GR I (RTS.cont_le GR R) R)).
-  Proof.
-  Admitted.
-
-End MC.
+Infix "^" := Pow.g : game_scope.
+Infix "^" := Pow.r : grel_scope.
