games/HComp.v
@@ -1,0 +1,105 @@
+Require Import ATS.
+Require Import MultiChannel.
+Require Import List.
+
+
+(** The flat composition of a family of alternating transition systems
+  switches between them with each opponent question, allowing one
+  component to proceed when all the others refuse. To match incoming
+  answers with the right component, we keep a stack of ids which
+  remembers what component asked what pending question. *)
+
+Module FComp.
+  Section ATS.
+    Context {GA GB : game} {I S K} (α : ats (GA ^ I) (GB ^ I) S K).
+
+    Definition state : Type := S * list I.
+    Definition cont : Type := K * list I.
+
+    Inductive step : state -> state -> Prop :=
+      | step_intro s s' stk :
+          ATS.step α s s' ->
+          step (s, stk) (s', stk).
+
+    Inductive suspend : state -> pmove GA GB * cont -> Prop :=
+      | suspend_q (m : question GA) i s k stk :
+          ATS.suspend α s (Pow.mkp i (inl m), k) ->
+          suspend (s, stk) (inl m, (k, i :: stk))
+      | suspend_a (m : answer GB) i s k stk :
+          ATS.suspend α s (Pow.mkp i (inr m), k) ->
+          suspend (s, stk) (inr m, (k, stk)).
+
+    Inductive resume : cont -> omove GA GB -> state -> Prop :=
+      | resume_q (m : question GB) i s k stk :
+          (forall j, ATS.refuse α k (j, m)) ->
+          ATS.resume α k (Pow.mko i (inr m)) s ->
+          resume (k, stk) (inr m) (s, stk)
+      | resume_a (m : answer GA) i s k stk :
+          ATS.resume α k (Pow.mko i (inl m)) s ->
+          resume (k, i :: stk) (inl m) (s, stk).
+
+    Inductive refuse : cont -> oqmove GA GB -> Prop :=
+      | refuse_intro (m : question GB) k stk :
+          (forall i, ATS.refuse α k (i, m)) ->
+          refuse (k, stk) m.
+
+    Definition of :=
+      ATS.Build_ats GA GB state cont step suspend resume refuse.
+
+  End ATS.
+End FComp.
+
+(** The resolution operator allows a component to interact with itself
+  by feeding back its own questions to it whenever possible. To make
+  sure we can direct back the reply to the right component, we keep a
+  stack of booleans indicating for each expected reply of the original
+  transition system, whether it will answer its own question or that
+  of the opponent. *)
+
+Module Res.
+  Section ATS.
+    Context {G S K} (α : ats G G S K).
+
+    Definition state : Type := S * list bool.
+    Definition cont : Type := K * list bool.
+
+    Inductive step : state -> state -> Prop :=
+      | step_int s s' stk :
+          ATS.step α s s' ->
+          step (s, stk) (s', stk)
+      | step_q (m : question G) s k s' stk :
+          ATS.suspend α s (inl m, k) ->
+          ATS.resume α k (inr m) s' ->
+          step (s, stk) (s', true :: stk)
+      | step_a (m : answer G) s k s' stk :
+          ATS.suspend α s (inr m, k) ->
+          ATS.resume α k (inl m) s' ->
+          step (s, true :: stk) (s', stk).
+
+    Inductive suspend : state -> pmove G G * cont -> Prop :=
+      | suspend_q (m : question G) s k stk :
+          ATS.suspend α s (inl m, k) ->
+          ATS.refuse α k m ->
+          suspend (s, stk) (inl m, (k, stk))
+      | suspend_a (m : answer G) s k stk :
+          ATS.suspend α s (inr m, k) ->
+          suspend (s, false :: stk) (inr m, (k, stk)).
+
+    Inductive resume : cont -> omove G G -> state -> Prop :=
+      | resume_q m k s stk :
+          ATS.resume α k (inr m) s ->
+          resume (k, stk) (inr m) (s, false :: stk)
+      | resume_a m k s stk :
+          ATS.resume α k (inl m) s ->
+          resume (k, stk) (inl m) (s, stk).
+
+    Inductive refuse : cont -> oqmove G G -> Prop :=
+      | refuse_intro k m stk :
+          ATS.refuse α k m ->
+          refuse (k, stk) m.
+
+    Definition of :=
+      ATS.Build_ats G G state cont step suspend resume refuse.
+
+  End ATS.
+End Res.
